chore(dafny): BKSA Mutate from HV-1 to HV-2 only Simple (#1458)
Co-authored-by: rishav-karanjit <karanjitrishav4@gmail.com>

AwsCryptographicMaterialProviders/dafny/AwsCryptographyKeyStoreAdmin/src/MutationStateStructures.dfy
@@ -3,6 +3,8 @@
 include "../Model/AwsCryptographyKeyStoreAdminTypes.dfy"
 include "../../../../libraries/src/JSON/API.dfy"
 include "MutationIndexUtils.dfy"
+include "KeyStoreAdminErrorMessages.dfy"
+include "CommitmentAndIndex.dfy"
 
 /** Mutation State Structures describe the Mutable Branch Key Properties that can be changed by Mutaiton. **/
 /** Methods here normialize these descriptions so they may be compared. **/
@@ -21,6 +23,7 @@ module {:options "/functionSyntax:4" } MutationStateStructures {
   import Types = AwsCryptographyKeyStoreAdminTypes
   import KeyStoreOperations = AwsCryptographyKeyStoreOperations
   import KeyStoreTypes = KeyStoreOperations.Types
+  import KeyStoreAdminErrorMessages
   import KmsArn
   import Structure
   import HVUtils = HierarchicalVersionUtils
@@ -30,10 +33,14 @@ module {:options "/functionSyntax:4" } MutationStateStructures {
   import JSONValues = JSON.Values
     // (Branch) Key Store Admin Imports
   import MutationIndexUtils
+  import CommitmentAndIndex
 
   const AWS_CRYPTO_EC := Structure.AWS_CRYPTO_EC
   const KMS_FIELD := Structure.KMS_FIELD
   const HV_FIELD := Structure.HIERARCHY_VERSION
+  const StringToHierarchyVersion := Structure.StringToHierarchyVersion
+  const HierarchyVersionToString := Structure.HierarchyVersionToString
+
   // Ensures
   // - if KMS ARN, Valid KMS ARN
   // - if EC, Valid non-empty EC, & not restricted field names
@@ -48,7 +55,10 @@ module {:options "/functionSyntax:4" } MutationStateStructures {
           &&  forall k <- input.TerminalEncryptionContext.value ::
                && |k| > 0 && |input.TerminalEncryptionContext.value[k]| > 0
                && input.TerminalEncryptionContext.value.Keys !! Structure.BRANCH_KEY_RESTRICTED_FIELD_NAMES)
-    && !(input.TerminalKmsArn.None? && input.TerminalEncryptionContext.None?)
+    && (input.TerminalHierarchyVersion.Some? ==>
+          input.TerminalHierarchyVersion.value.v1? || input.TerminalHierarchyVersion.value.v2?
+       )
+    && !(input.TerminalKmsArn.None? && input.TerminalEncryptionContext.None? && input.TerminalHierarchyVersion.None?)
   }
 
   /**
@@ -91,54 +101,6 @@ module {:options "/functionSyntax:4" } MutationStateStructures {
     }
   }
 
-  /**
-     The Commitment & Index are persisted to the storage by Initialize.
-     The Commitment & Index are read by Apply.
-     The Index is updated by Apply.
-     Both are deleted when the Mutation is completed by Apply.
-   */
-  datatype CommitmentAndIndex = CommitmentAndIndex(
-    Commitment: KeyStoreTypes.MutationCommitment,
-    Index: KeyStoreTypes.MutationIndex
-  )
-  {
-    /** 
-      The Commitment & Index MUST always have the same Identifier & UUID. 
-      They MAY NOT have the same CreateTime. 
-    */
-    predicate ValidState()
-    {
-      && Commitment.Identifier == Index.Identifier
-      && Commitment.UUID == Index.UUID
-      && ValidCommitment?(Commitment)
-      && ValidIndex?(Index)
-    }
-    // TODO-HV-2-FOLLOW : See if we can drop ValidUTF8
-    predicate ValidUTF8()
-    {
-      && ValidCommitment?(Commitment)
-      && ValidIndex?(Index)
-    }
-  }
-
-  predicate ValidCommitment?(
-    Commitment: KeyStoreTypes.MutationCommitment
-  ) {
-    && UTF8.ValidUTF8Seq(Commitment.Original)
-    && UTF8.ValidUTF8Seq(Commitment.Terminal)
-    && UTF8.ValidUTF8Seq(Commitment.Input)
-    && 0 < |Commitment.Identifier|
-    && 0 < |Commitment.UUID|
-  }
-
-  predicate ValidIndex?(
-    Index: KeyStoreTypes.MutationIndex
-  ) {
-    && 0 < |Index.Identifier|
-    && 0 < |Index.UUID|
-    && UTF8.ValidUTF8Seq(Index.PageIndex)
-  }
-
   // Pre-HV-2 Mutations did not track Hierarchy Version;
   // therefore, HV MAY NOT be present in a Mutation Commitment.
   // If HV is not present, we KNOW it is HV1.
@@ -150,7 +112,7 @@ module {:options "/functionSyntax:4" } MutationStateStructures {
     requires MutablePropertiesJson?(deserializedMutableProperties).Pass?
   {
     if |deserializedMutableProperties.obj| == 3
-    then HVUtils.StringToHierarchyVersion(deserializedMutableProperties.obj[2].1.str)
+    then StringToHierarchyVersion(deserializedMutableProperties.obj[2].1.str)
     else KeyStoreTypes.HierarchyVersion.v1
   }
 
@@ -166,7 +128,7 @@ module {:options "/functionSyntax:4" } MutationStateStructures {
     requires MutablePropertiesJson?(deserializedInput).Pass?
   {
     if |deserializedInput.obj| == 3 && deserializedInput.obj[2].0 == HV_FIELD && deserializedInput.obj[2].1.String?
-    then Some(HVUtils.StringToHierarchyVersion(deserializedInput.obj[2].1.str))
+    then Some(StringToHierarchyVersion(deserializedInput.obj[2].1.str))
     else None
   }
 
@@ -251,7 +213,7 @@ module {:options "/functionSyntax:4" } MutationStateStructures {
       else JSONValues.Null;
     var hv: JSONValues.JSON :=
       if Mutations.TerminalHierarchyVersion.Some?
-      then JSONValues.JSON.String(HVUtils.HierarchyVersionToString(Mutations.TerminalHierarchyVersion.value))
+      then JSONValues.JSON.String(HierarchyVersionToString(Mutations.TerminalHierarchyVersion.value))
       else JSONValues.Null;
     // TODO-HV-2-M2 : Ensure that pre-HV-1 Mutation Commitments deserialize
     // such commitments will not have the new HV field
@@ -290,7 +252,7 @@ module {:options "/functionSyntax:4" } MutationStateStructures {
       else None;
     var hv: Option<KeyStoreTypes.HierarchyVersion> :=
       if |MutationsJson.obj| == 3 && MutationsJson.obj[2].1.String?
-      then Some(HVUtils.StringToHierarchyVersion(MutationsJson.obj[2].1.str))
+      then Some(StringToHierarchyVersion(MutationsJson.obj[2].1.str))
       else None;
     var input
       := Types.Mutations(
@@ -344,14 +306,14 @@ module {:options "/functionSyntax:4" } MutationStateStructures {
            [
              (AWS_CRYPTO_EC, EncryptionContextStringToJSON(MutationToApply.Original.customEncryptionContext)),
              (KMS_FIELD, JSONValues.JSON.String(MutationToApply.Original.kmsArn)),
-             (HV_FIELD, JSONValues.JSON.String(HVUtils.HierarchyVersionToString(MutationToApply.Original.hierarchyVersion)))
+             (HV_FIELD, JSONValues.JSON.String(HierarchyVersionToString(MutationToApply.Original.hierarchyVersion)))
            ]);
     var TerminalJson
       := JSONValues.Object(
            [
              (AWS_CRYPTO_EC, EncryptionContextStringToJSON(MutationToApply.Terminal.customEncryptionContext)),
              (KMS_FIELD, JSONValues.JSON.String(MutationToApply.Terminal.kmsArn)),
-             (HV_FIELD, JSONValues.JSON.String(HVUtils.HierarchyVersionToString(MutationToApply.Terminal.hierarchyVersion)))
+             (HV_FIELD, JSONValues.JSON.String(HierarchyVersionToString(MutationToApply.Terminal.hierarchyVersion)))
            ]);
 
     var InputJson := InputMutationsToJson(MutationToApply.Input);
@@ -420,13 +382,13 @@ module {:options "/functionSyntax:4" } MutationStateStructures {
   // TODO-HV-2-M2 : Ensure that pre-HV-1 Mutation Commitments deserialize
   // such commitments will not have the new HV field
   function DeserializeMutation(
-    commitmentAndIndex: CommitmentAndIndex
+    commitmentAndIndex: CommitmentAndIndex.CommitmentAndIndex
   ): (output: Result<MutationToApply, Types.Error>)
-    requires commitmentAndIndex.ValidState()
+    requires commitmentAndIndex.ValidIDs() && commitmentAndIndex.ValidUTF8()
     ensures output.Success? ==> output.value.ValidState()
   {
-    var commitment := commitmentAndIndex.Commitment;
-    var index := commitmentAndIndex.Index;
+    var commitment := commitmentAndIndex.commitment;
+    var index := commitmentAndIndex.index;
     var OriginalJson: JSONValues.JSON :- JSON.Deserialize(commitment.Original).MapFailure(
                                            (e: JSONErrors.DeserializationError)
                                            => Types.KeyStoreAdminException(
