AwsCryptographicMaterialProviders/dafny/AwsCryptographyKeyStoreAdmin/src/KeyStoreAdminErrorMessages.dfy
@@ -5,6 +5,67 @@ module {:options "/functionSyntax:4" } KeyStoreAdminErrorMessages {
   const NO_MUTATE_TO_HV_1: string :=
     "At this time, a Mutation cannot change a Branch Key from HV-2 to HV-1. The request dictated 'TerminalHierarchyVersion := v1' and was therefore rejected. Remove the 'TerminalHierarchyVersion' parameter or set it to at least 'v2'."
 
-  const UNSUPPORTED_KEYMANAGEMENTSTRATEGY_HV_2: string :=
+  const UNSUPPORTED_KEY_MANAGEMENT_STRATEGY :=
+    "Unsupported KeyManagementStrategy."
+    + " Only KeyManagementStrategy.AwsKmsReEncrypt and KeyManagementStrategy.AwsKmsDecryptEncrypt"
+    + " is allowed when terminal hierarchical version is 1."
+    + " Only KeyManagementStrategy.kmsSimple is allowed when terminal hierarchical version is 2."
+
+  const UNSUPPORTED_KEY_MANAGEMENT_STRATEGY_HV_2: string :=
     "Only KeyManagementStrategy.AwsKmsSimple is allowed when mutating to hv-2."
+
+  const UNSUPPORTED_DOWNGRADE_HV: string :=
+    "Mutation which Downgrades hierarchical version (example: from v2 to v1) is not supported."
+
+  function TokenAndMutationCommitmentDisagree(
+    mutationTokenIdentifier: string,
+    mutationCommitmentUUID: string,
+    mutationTokenUUID: string
+  ): string
+  {
+    "The Token and the Mutation Commitment read from storage disagree."
+    + " This indicates that the Token is for a different Mutation than the one in-flight."
+    + " A possible cause is this token is from an earlier Mutation that already finished?"
+    + " Branch Key ID: " + mutationTokenIdentifier + ";"
+    + " Mutation Commitment UUID: " + mutationCommitmentUUID + ";"
+    + " Token UUID: " + mutationTokenUUID + ";"
+  }
+
+  function NoMutationInFlight(
+    mutationTokenIdentifier: string
+  ): string
+  {
+    "No Mutation is in-flight for this Branch Key ID " + mutationTokenIdentifier + " ."
+  }
+
+  function NoMutationIndexExists(
+    mutationTokenIdentifier: string
+  ): string
+  {
+    "No Mutation Index exists for this in-flight mutation of Branch Key ID " + mutationTokenIdentifier + " ."
+  }
+
+  function IndexAndCommitmentUUIDDisagree(
+    nameonly indexUUID: string,
+    nameonly commitmentUUID: string
+  ): string
+  {
+    "Mutation Index or Mutation Commitment is corrupted; their UUIDs MUST be equal."
+    + " MUTATION_INDEX uuid: " + indexUUID + ";"
+    + " MUTATION_COMMITMENT uuid: " + commitmentUUID + ";"
+  }
+
+  function IndexAndCommitmentBKIDDisagree(
+    nameonly indexBKID: string,
+    nameonly commitmentBKID: string
+  ): string
+  {
+    "Mutation Index or Mutation Commitment is corrupted; their Branch Key IDs MUST be equal."
+    + " MUTATION_INDEX Branch Key ID: " + indexBKID + ";"
+    + " MUTATION_COMMITMENT Branch Key ID: " + commitmentBKID + ";"
+  }
+
+  const INVALID_COMMITMENT_UTF8 := "Mutation Commitment read from storage contains invalid UTF-8."
+  const INVALID_INDEX_UTF8 := "Mutation Index read from storage contains invalid UTF-8."
+  const INVALID_COMMITMENT_UUID := "Mutation Commitment read from storage has an invalid UUID."
 }
